Updates

intermediate2/Zeta.Intermediate.Store.fst
@@ -1431,6 +1431,30 @@ let puts_store (#vcfg:_)
   : vstore vcfg
   = admit()
 
+let puts_preserves (#vcfg:_)
+  (st: vstore vcfg)
+  (ss: S.seq (slot_id vcfg))
+  (ws: S.seq (app_value_nullable vcfg.app.adm))
+  (s: slot_id vcfg)
+  : Lemma (ensures (let st_ = puts_store st ss ws in
+                    inuse_slot st s = inuse_slot st_ s /\
+                    inuse_slot st s ==> (
+                      stored_key st s = stored_key st_ s /\
+                      add_method_of st s = add_method_of st_ s /\
+                      points_to_info st s Left = points_to_info st_ s Left /\
+                      points_to_info st s Right = points_to_info st_ s Right)))
+  = admit()
+
+let puts_preserves_non_ref (#vcfg:_)
+  (st: vstore vcfg)
+  (ss: S.seq (slot_id vcfg))
+  (ws: S.seq (app_value_nullable vcfg.app.adm))
+  (s: slot_id vcfg)
+  : Lemma (ensures (let st_ = puts_store st ss ws in
+                    not (S.mem s ss) ==>
+                    get_slot st s = get_slot st_ s))
+  = admit()
+
 let puts_preserve_ismap (#vcfg:_)
   (st: ismap_vstore vcfg)
   (ss: S.seq (slot_id vcfg))
